Primera versión de swapping.

src/Renaming.thy
@@ -2,28 +2,72 @@ theory Renaming imports Formula begin
 
 section\<open>Renaming of free variables\<close>
 
+definition autom :: "i \<Rightarrow> o" where
+  "autom(f) == function(f) \<and> f = converse(f)"
+
 text\<open>TODO: this can be generalized to any pair of functions.\<close>
-(*
 definition 
   perm_n :: "[i,i] \<Rightarrow> i" where
   "perm_n(m,f) == \<lambda>n \<in> succ(m)  . if n=0 then 0 else succ(f`pred(n))"
 
+lemma perm_n0 : "perm_n(m,f)`0 = 0"
+  by(unfold perm_n_def,simp)
+
+lemma perm_nS : "succ(x) \<in> succ(m) \<Longrightarrow> perm_n(m,f)`succ(x) = succ(f`x)"
+  by(unfold perm_n_def,simp)
+
+    
 lemma nat_succ [TC]: "m \<in> nat \<Longrightarrow> n\<in>nat \<Longrightarrow> n \<in> m \<Longrightarrow> succ(n) \<in> succ(m)"
   by (rule Ord_succ_mem_iff [THEN iffD2],auto)
 
+lemma nat_succE : "m \<in> nat \<Longrightarrow>  succ(n) \<in> succ(m) \<Longrightarrow> n \<in> m"
+  by (drule_tac j="succ(m)" in ltI,auto,erule ltD)
+    
 lemma zero_in [TC]: "m \<in> nat \<Longrightarrow> 0\<in>succ(m)"
   by (rule ltD,auto)
+    
+lemma ltI_neg : "x \<in> nat \<Longrightarrow> j \<le> x \<Longrightarrow> j \<noteq> x \<Longrightarrow> j < x"
+  by (insert le_iff,auto)
+
+lemma leD_cases [simp] : "x \<in> nat \<Longrightarrow> j \<le> x \<Longrightarrow> j = x \<or> j < x"
+  by(insert le_iff,auto)
     
 lemma succ_pred_eq [simp] :  "m \<in> nat \<Longrightarrow> m \<noteq> 0  \<Longrightarrow> succ(pred(m)) = m"
  by (erule_tac n="m" in natE,auto)
 
 lemma in_n_in_nat :  "m \<in> nat \<Longrightarrow> n \<in> m \<Longrightarrow> n \<in> nat"
  by(rule_tac A="m" in subsetD,erule naturals_subset_nat,assumption)
-   
+
+lemma le_in_nat [TC] :  "m \<in> nat \<Longrightarrow> n \<le> m \<Longrightarrow> n \<in> nat"
+  apply (case_tac "m=n",simp)
+  apply(frule ltI_neg,auto,erule_tac m="m" in in_n_in_nat,erule ltD)
+done
+    
 lemma in_succ_in_nat [TC] : "m \<in> nat \<Longrightarrow> n \<in> succ(m) \<Longrightarrow> n \<in> nat"
   apply(rule_tac A="succ(m)" in subsetD,rule naturals_subset_nat)
   apply(rule nat_succ_iff [THEN iffD2],assumption+)
 done
+
+lemma succ_leI : "j \<le> n \<Longrightarrow> succ(j) \<le> succ(n)"
+  by (auto)
+    
+lemma succ_ltI : "n \<in> nat \<Longrightarrow> succ(j) < n \<Longrightarrow> j < n"
+  apply (rule_tac j="succ(j)" in lt_trans,rule le_refl,rule Ord_succD)
+  apply (rule nat_into_Ord,erule in_n_in_nat,erule ltD,simp)
+done
+
+lemma succ_In : "n \<in> nat \<Longrightarrow> succ(j) \<in> n \<Longrightarrow> j \<in> n"
+ by (rule ltD,rule succ_ltI,simp,rule ltI,auto)
+    
+  
+lemma succ_leD : "n \<in> nat \<Longrightarrow> succ(j) \<le> n \<Longrightarrow> j \<le> n"
+  apply (subgoal_tac "succ(j) \<in> nat")
+  apply (rule_tac j="succ(j)" in le_trans,simp,assumption)
+  apply (erule le_in_nat,simp)
+  done
+    
+lemma succpred_leI : "n \<in> nat \<Longrightarrow>  n \<le> succ(pred(n))"
+  by (erule natE,simp+)
     
 lemma perm_n_bd [TC] : "m \<in> nat \<Longrightarrow> n\<in> nat \<Longrightarrow> 
       f \<in> m \<rightarrow> m \<Longrightarrow> n \<in> succ(m) \<Longrightarrow> (if n = 0 then 0 else succ(f`pred(n))) \<in> succ(m)"
@@ -75,18 +119,219 @@ lemma perm_n_bij [TC] : "m \<in> nat \<Longrightarrow> f \<in> bij(m,m) \<Longri
   apply(simp,simp,erule right_inverse_bij)
   apply(rule Ord_succ_mem_iff [THEN iffD1],simp,assumption)
 done
-    
-definition perm_list :: "[i,i,i] \<Rightarrow> i" where
-  "perm_list(f,l,i) ==  nat_rec(i,Nil,\<lambda> a e . e@[nth(f`a,l)])"
 
-(* TODO : nice property *)
-(*
-lemma perm_perm : "\<lbrakk> l \<in> list(A) ; f \<in> bij(length(l),length(l)) \<rbrakk> \<Longrightarrow>
-   perm_list(converse(f),perm_list(f,l,length(l)),length(l)) = l"
-  apply(induct_tac l,simp,unfold perm_list_def)
-  apply(rule nat_rec_0)
-  sorry
-*)  
+lemma conv_perm_n0 : "m \<in> nat \<Longrightarrow> f \<in> bij(m,m) \<Longrightarrow> converse(perm_n(m,f))`0 = 0"
+  by(subst (1) perm_n0[symmetric],subst left_inverse_bij,erule perm_n_bij,auto)
+
+    
+lemma perm_nRel : "m \<in> nat \<Longrightarrow> f\<in>bij(m,m) \<Longrightarrow> x \<in> m \<Longrightarrow>
+  <succ(x),y> \<in> perm_n(m,f) \<Longrightarrow> y=succ(f`x)" 
+  apply(subgoal_tac "perm_n(m,f)`(succ(x)) = succ(f`x)")
+  prefer 2 apply(rule perm_nS,rule nat_succ,simp,erule in_n_in_nat,simp,simp)
+  apply(drule function_apply_equality)
+   apply(rule fun_is_function,rule bij_is_fun,rule perm_n_bij,simp+)
+done
+
+lemma funcI : "f \<in> A \<rightarrow> B \<Longrightarrow> a \<in> A \<Longrightarrow> b= f ` a \<Longrightarrow> \<langle>a, b\<rangle> \<in> f"
+  by(simp,rule apply_Pair,simp+)
+
+lemma conv_perm_s : "m \<in> nat \<Longrightarrow> f \<in> bij(m,m) \<Longrightarrow> succ(n) \<in> succ(m) \<Longrightarrow>
+    (converse(perm_n(m, f))`succ(n) = perm_n(m, converse(f))`succ(n))"  
+  apply(rule function_apply_equality,rule converseI)
+  apply(subst perm_nS,simp)
+  apply(rule funcI,rule perm_n_tc,simp,erule bij_is_fun)
+    prefer 2 apply(subst perm_nS)
+    prefer 2 apply(subst right_inverse_bij,simp+)
+    apply(rule nat_succE,simp+,rule nat_succ,simp)
+    apply(rule in_n_in_nat,simp)
+   apply(rule apply_type,rule bij_is_fun,erule bij_converse_bij,rule nat_succE,simp+)
+   apply(rule apply_type,rule bij_is_fun,erule bij_converse_bij,rule nat_succE,simp+)
+   apply(subgoal_tac "converse(perm_n(m,f)) \<in> bij(succ(m),succ(m))")
+   apply(drule bij_is_fun[of "converse(perm_n(m,f))"],drule Pi_iff[THEN iffD1],auto)
+  done
+
+lemma conv_perm_ap : "m \<in> nat \<Longrightarrow> f \<in> bij(m,m) \<Longrightarrow> n \<in> succ(m) \<Longrightarrow>
+    (converse(perm_n(m, f))`n) = perm_n(m, converse(f))`n"  
+  apply(rule_tac n="n" in natE,rule in_n_in_nat,erule nat_succI,simp)
+  apply(simp add: conv_perm_n0 perm_n0,simp)
+  apply(rule conv_perm_s,simp+)
+  done
+    
+lemma conv_perm : "m \<in> nat \<Longrightarrow> f \<in> bij(m,m) \<Longrightarrow> 
+    converse(perm_n(m, f)) = perm_n(m, converse(f))"
+  apply(rule fun_extension,rule bij_is_fun,rule bij_converse_bij,rule perm_n_bij,simp+)
+  apply(rule bij_is_fun,rule perm_n_bij,simp+,rule conv_perm_ap,simp+)
+done
+    
+definition 
+  tabulate :: "[i,i] \<Rightarrow> i" where 
+  "tabulate(f,i) = nat_rec(i,Nil, \<lambda> j l . l@[f`j])" 
+ 
+lemma tab_tc_aux [rule_format] : "i \<in> nat \<Longrightarrow> 
+  \<forall> m f . i\<le> m \<longrightarrow> f \<in> m \<rightarrow> A \<longrightarrow> tabulate(f,i) \<in> list(A)"
+  apply(erule_tac n="i" in nat_induct)
+  apply(clarsimp,unfold tabulate_def,subst nat_rec_0,simp)
+  apply(rename_tac i)
+  apply(clarsimp,subst nat_rec_succ,simp,rule app_type)
+  prefer 2 apply(simp,erule apply_type,erule ltD)
+  apply(rename_tac n g)
+  apply(subgoal_tac "i\<le>n")
+   prefer 2 apply(erule leI)
+  apply(auto)
+done
+
+lemma tab_tc [TC] : "\<lbrakk> j \<in> nat ;  f \<in> j \<rightarrow> A \<rbrakk> \<Longrightarrow> 
+                       tabulate(f,j) \<in> list(A)"
+ by (rule tab_tc_aux,assumption,auto)
+
+lemma tab_succ : "\<lbrakk> j \<in> nat ; f \<in> n \<rightarrow> A \<rbrakk> \<Longrightarrow> 
+                       tabulate(f,succ(j)) = tabulate(f,j)@[f`j]"
+   by(unfold tabulate_def,subst nat_rec_succ,assumption+,simp)
+
+lemma tab_length : "\<lbrakk> j \<in> nat \<rbrakk> \<Longrightarrow> \<forall> n . n \<in> nat \<longrightarrow> j \<le> n \<longrightarrow> (\<forall> f . (f \<in> n \<rightarrow> A) \<longrightarrow> 
+                       length(tabulate(f,j)) = j)"
+  apply(erule nat_induct)
+  apply(unfold tabulate_def,subst nat_rec_0,(rule allI,rule impI)+,simp)
+  apply((rule allI,rule impI)+,subst nat_rec_succ,assumption)
+  apply(rule impI,rule allI,rule impI)
+  apply(subst length_app,fold tabulate_def,rule tab_tc_aux,simp)
+   apply(rule_tac j="succ(x)" in le_trans,simp,assumption+,simp)
+   apply(rule apply_type,assumption,erule ltD,simp)
+  apply(subst natify_ident,rule length_type,rule tab_tc_aux,assumption)
+   apply(erule leI,assumption)
+  apply(subgoal_tac "x\<le>n",auto,erule leI)
+done
+
+lemma tab_length2 : "\<lbrakk> j \<in> nat ; n \<in> nat ;  f \<in> n \<rightarrow> A ; j < n \<rbrakk> \<Longrightarrow> 
+                       length(tabulate(f,j)) = j"
+  by(subgoal_tac "j\<le>n",insert tab_length,simp,erule leI)
+
+
+definition nth_i :: "i \<Rightarrow> i" where
+  "nth_i(l) == \<lambda> n\<in>length(l).nth(n,l)"
+
+lemma nth_eq : "l \<in> list(A) \<Longrightarrow> n \<in> length(l) \<Longrightarrow> nth_i(l)`n=nth(n,l)"
+  by(unfold nth_i_def,simp)
+    
+lemma nth_i_type : "l \<in> list(A) \<Longrightarrow> nth_i(l) \<in> length(l) \<rightarrow> A"
+  by (unfold nth_i_def,rule lam_type,rule nth_type,auto,rule ltI,simp,rule nat_into_Ord,auto)
+
+definition perm_list :: "[i,i] \<Rightarrow> i" where
+ "perm_list(f,l) ==tabulate(nth_i(l) O f,length(l))"
+
+
+lemmas natEin = natE [OF lt_nat_in_nat]  
+
+lemma trich_nat : "\<lbrakk> m \<in> nat ; n \<le> m ; n \<noteq> m ; \<not> n < m \<rbrakk> \<Longrightarrow> P"
+  apply(subgoal_tac "Ord(n)" "Ord(m)" "\<not> m < n")
+  apply(rule_tac i="n" and j="m" in Ord_linear_lt,assumption+,blast+)
+  apply(erule le_imp_not_lt,erule nat_into_Ord)
+  apply(rule nat_into_Ord[OF le_in_nat],assumption+)
+  done
+    
+lemma nth_tab_gen: 
+  "m \<in>nat \<Longrightarrow> \<forall> n . n \<in> nat \<longrightarrow> m \<le> n \<longrightarrow> (\<forall> f . (f \<in> n \<rightarrow> A \<longrightarrow>(
+   \<forall> j . j < m \<longrightarrow> nth(j,tabulate(f,m)) = f`j)))" 
+  apply(erule nat_induct,simp)
+  apply(rule allI,(rule impI)+)+
+  apply(case_tac "j=x")
+  apply(simp,unfold tabulate_def,subst nat_rec_succ,assumption)
+   apply(fold tabulate_def,subst nth_append)
+  apply(rule_tac i="x" and m="n" and A="A" in tab_tc_aux,assumption,erule leI,assumption+)
+  apply(simp add: tab_length2,blast)
+  apply(subst tab_succ,assumption+,simp,subst nth_append) 
+    apply(rule_tac i="x" and m="n" and A="A" in tab_tc_aux,assumption,erule leI,assumption+)
+    apply(erule_tac m="x" in le_in_nat,assumption)
+  apply(simp add: tab_length2,rule conjI)
+  prefer 2 apply(rule impI,erule_tac m="x" and n="j" in trich_nat,assumption+)
+  apply(subgoal_tac "x\<le>n",blast,erule leI)
+  done
+
+lemma nth_tab: 
+  "j \<in> nat \<Longrightarrow> m \<in> nat \<Longrightarrow> f \<in> m \<rightarrow> A \<Longrightarrow> j \<in> m \<Longrightarrow> nth(j,tabulate(f,m)) = f`j" 
+ by(subgoal_tac "j<m",insert nth_tab_gen,auto,erule ltI,erule nat_into_Ord)
+ 
+lemma nth_after_type [TC]: 
+  "l\<in>list(A) \<Longrightarrow> f \<in> length(l) \<rightarrow> length(l) \<Longrightarrow>
+   j < length(l) \<Longrightarrow> nth(f`j,l) \<in> A" 
+  apply(subgoal_tac "f`j < length(l)")
+   apply(erule nth_type,assumption)
+  apply(rule ltI,erule apply_type,erule ltE,auto)
+done
+
+
+lemma perm_list_tc : " l \<in> list(A) \<Longrightarrow> 
+    f\<in> bij(length(l),length(l)) \<Longrightarrow> 
+    perm_list(f,l) \<in> list(A)"
+  apply(unfold perm_list_def,rule tab_tc,simp)
+  apply(rule comp_fun,erule bij_is_fun,erule nth_i_type )
+done
+
+lemma perm_list_length : " l \<in> list(A) \<Longrightarrow> 
+    f\<in> bij(length(l),length(l)) \<Longrightarrow> 
+    length(perm_list(f,l)) = length(l)"
+  apply(unfold perm_list_def,subst tab_length,simp,rule length_type,assumption,simp)
+  apply(rule comp_fun,erule bij_is_fun,rule nth_i_type,simp+)
+done
+    
+lemma nth_tab_perm : "\<lbrakk> m \<in> nat ; h \<in> m \<rightarrow> A ; f \<in> bij(m,m) ; n \<in> m \<rbrakk> \<Longrightarrow>
+  nth(converse(f)`n,tabulate(h O f,m)) = h`n"
+ apply(subst nth_tab,auto,rule in_n_in_nat,assumption,rule apply_type)    
+ apply(rule bij_is_fun[OF bij_converse_bij],assumption+)
+ apply(rule comp_fun,rule bij_is_fun,assumption+)
+ apply(rule apply_type,rule bij_is_fun[OF bij_converse_bij],assumption+)
+ apply(subst comp_fun_apply,erule bij_is_fun)
+ apply(rule apply_type,rule bij_is_fun[OF bij_converse_bij],assumption+)
+ apply(subst right_inverse_bij,auto)
+done
+
+lemma bij_is_function : "f\<in>bij(A,A) \<Longrightarrow> function(f)"
+  by(drule bij_is_fun,drule Pi_iff[THEN iffD1],simp)
+
+lemma perm_list_eq : "\<lbrakk> l \<in> list(A) ; a \<in> A ; f \<in> bij(length(l),length(l)) \<rbrakk> \<Longrightarrow> 
+  perm_list(perm_n(length(l),f), Cons(a, l)) = Cons(a,perm_list(f,l))"  
+  apply(rule nth_equalityI)
+  apply(rule perm_list_tc,simp,simp+,rule perm_list_tc,simp+)
+  apply(subst perm_list_length,simp,(subst length.simps(2))+)
+  apply(rule perm_n_bij,simp+,subst perm_list_length,simp+)
+  apply(subst (asm) perm_list_length,simp,(subst length.simps(2))+)
+  apply(rule perm_n_bij,simp+)
+  apply(erule natE,simp)
+  apply(unfold perm_list_def)
+  apply(subst nth_tab,simp+)
+  apply(rule comp_fun,rule perm_n_tc,simp,erule bij_is_fun)
+  apply(subst length.simps(2)[symmetric],rule nth_i_type,simp+)
+  apply(subst comp_fun_apply) 
+  apply(rule perm_n_tc,simp,erule bij_is_fun,simp)
+  apply(subst perm_n0,subst nth_eq,simp+)
+  apply(subst nth_tab,simp+)
+  apply(rule comp_fun,rule perm_n_tc,simp,erule bij_is_fun)
+  apply(subst length.simps(2)[symmetric],rule nth_i_type,simp+)
+  apply(rule ltD,simp)
+  apply(subst comp_fun_apply,rule perm_n_tc,simp,erule bij_is_fun)
+  apply(rule ltD,simp)
+  apply(subst nth_eq,simp+)
+  apply(rule apply_type,rule perm_n_tc,simp,rule bij_is_fun,simp,rule ltD,simp)
+  apply(subst perm_nS,rule ltD,simp,subst nth_Cons)
+  apply(rule in_n_in_nat,rule length_type,simp,rule apply_type,rule bij_is_fun,simp,erule ltD)
+  apply(subst nth_tab,simp+)  
+  apply(rule comp_fun,erule bij_is_fun)
+  apply(rule nth_i_type,simp+,rule ltD,simp)
+  apply(subst comp_fun_apply,erule bij_is_fun,rule ltD,simp)
+  apply(subst nth_eq,simp+,rule apply_type,erule bij_is_fun,rule ltD,simp+)
+done
+    
+lemma nth_perm : "\<lbrakk> l \<in> list(A) ; f \<in> bij(length(l),length(l)) ; n \<in> length(l) \<rbrakk> \<Longrightarrow>
+  nth(converse(f)`n,perm_list(f,l)) = nth(n,l)"
+  by (unfold perm_list_def,subst nth_tab_perm,simp,erule nth_i_type,simp+,rule nth_eq,auto) 
+
+lemma nth_perm1 : "\<lbrakk> l \<in> list(A) ; f \<in> bij(length(l),length(l)) ; n \<in> length(l) \<rbrakk> \<Longrightarrow>
+  nth(n,perm_list(f,l)) = nth(f`n,l)"
+  apply (unfold perm_list_def,subst nth_tab,rule in_n_in_nat,(erule length_type,simp)+)
+  apply(erule length_type,rule comp_fun,erule bij_is_fun,erule nth_i_type,simp)
+  apply(subst comp_fun_apply,erule bij_is_fun,simp,erule nth_eq,rule apply_type,erule bij_is_fun,simp)
+done
+    
 consts   rename :: "i=>i"
 primrec
   "rename(Member(x,y)) =
@@ -105,29 +350,42 @@ primrec
 lemma app_bij [TC] : "f \<in> bij(A,B) \<Longrightarrow> a \<in> A \<Longrightarrow> f`a \<in> B"
   by (frule  bij_is_fun,auto)
 
-lemma succ_in [TC] : "succ(x) < y  \<Longrightarrow> x \<in> y"
- by (rule ltD,rule succ_leE,erule leI)
-
-lemma nat_ord [TC] : "n \<in> nat \<Longrightarrow> Ord(n)"
- by (auto)
+lemma succ_in [TC] : "succ(x) \<le> y  \<Longrightarrow> x \<in> y"
+ by (auto,rule ltD) 
   
-lemmas Un_least_lt_iffn [TC] =  Un_least_lt_iff [OF nat_ord nat_ord]
+lemmas Un_least_lt_iffn [TC] =  Un_least_lt_iff [OF nat_into_Ord nat_into_Ord]
 
 lemma pred_le2 : "n\<in> nat \<Longrightarrow> m \<in> nat \<Longrightarrow> pred(n) < m \<Longrightarrow> n \<le> m"
   by(subgoal_tac "n\<in>nat",rule_tac n="n" in natE,auto)
 
-lemma un_leD1 : "i \<in> nat \<Longrightarrow> j\<in> nat \<Longrightarrow> k \<in> nat \<Longrightarrow>  i \<union> j < k \<Longrightarrow> i < k"   
+lemma un_leD1 : "i \<in> nat \<Longrightarrow> j\<in> nat \<Longrightarrow> k \<in> nat \<Longrightarrow>  i \<union> j \<le> k \<Longrightarrow> i \<le> k"   
   by (rule conjunct1,rule  iffD1, rule_tac j="j" in Un_least_lt_iffn,assumption+)
 
 lemma un_leD2 : "i \<in> nat \<Longrightarrow> j\<in> nat \<Longrightarrow> k \<in> nat \<Longrightarrow>  i \<union> j < k \<Longrightarrow> j < k"   
   by (rule conjunct2,rule  iffD1, rule_tac j="j" in Un_least_lt_iffn,assumption+)
 
-lemma ren_tc [TC] : "p \<in> formula \<Longrightarrow> 
-      (\<forall> n f . n \<in> nat \<longrightarrow>f \<in> bij(n,n) \<longrightarrow> arity(p) < n \<longrightarrow> rename(p)`n`f \<in> formula)"
+lemma ren_mem [simp] : "\<lbrakk> i \<in> nat ; j\<in>nat ; n \<in> nat ; f \<in> bij(n,n)\<rbrakk> \<Longrightarrow> 
+  rename(Member(i,j))`n`f = Member(f`i,f`j)"
+  by (auto)
+
+lemma ren_eq [simp] : "\<lbrakk> i \<in> nat ; j\<in>nat ; n \<in> nat ; f \<in> bij(n,n)\<rbrakk> \<Longrightarrow> 
+  rename(Equal(i,j))`n`f = Equal(f`i,f`j)"
+  by (auto)
+
+lemma ren_nand [simp] : "\<lbrakk> p \<in> formula ; q\<in>formula ; n \<in> nat ; f \<in> bij(n,n)\<rbrakk> \<Longrightarrow> 
+  rename(Nand(p,q))`n`f = Nand(rename(p)`n`f,rename(q)`n`f)"
+  by (auto)
+
+lemma ren_forall [simp] : "\<lbrakk> p \<in> formula ; n \<in> nat ; f \<in> bij(n,n)\<rbrakk> \<Longrightarrow> 
+  rename(Forall(p))`n`f = Forall(rename(p)`succ(n)`perm_n(n,f))"
+  by (auto)
+    
+lemma ren_tc : "p \<in> formula \<Longrightarrow> 
+      (\<forall> n f . n \<in> nat \<longrightarrow>f \<in> bij(n,n) \<longrightarrow> arity(p) \<le> n \<longrightarrow> rename(p)`n`f \<in> formula)"
   apply (induct_tac p,simp_all)
   apply (clarsimp,subgoal_tac "f`x \<in> nat \<and> f`y \<in> nat",blast,rule conjI)
-  apply(rule_tac m="n" in in_n_in_nat,assumption)
-  apply(erule app_bij, rule succ_in,rule_tac j="succ(y)" in un_leD1,simp+)
+  apply(rule_tac m="n" in in_n_in_nat,assumption,erule app_bij)
+  apply(rule succ_in,rule_tac j="succ(y)"  in un_leD1,simp+)
   apply(rule_tac m="n"  in in_n_in_nat,assumption) 
   apply(erule app_bij, rule succ_in,rule_tac i="succ(x)" in un_leD2,simp+)
   apply (clarsimp,subgoal_tac "f`x \<in> nat \<and> f`y \<in> nat",blast,rule conjI)
@@ -135,86 +393,248 @@ lemma ren_tc [TC] : "p \<in> formula \<Longrightarrow>
   apply(erule app_bij, rule succ_in,rule_tac j="succ(y)" in un_leD1,simp+)
   apply(rule_tac m="n"  in in_n_in_nat,assumption) 
   apply(erule app_bij, rule succ_in,rule_tac i="succ(x)" in un_leD2,simp+)    
-  apply(auto,subgoal_tac "arity(p)<n",simp)
-  apply(rule conjunct1,rule  iffD1,rule Un_least_lt_iff,auto)
-  apply(subgoal_tac "arity(q)<n",simp)
-  apply(rule conjunct2,rule  iffD1,rule Un_least_lt_iff,auto)
+  apply(auto,subgoal_tac "arity(p)\<le>n",simp)
+    apply(rule Un_least_lt_iff[THEN iffD1[THEN conjunct1]])
+      apply(rule nat_into_Ord,erule arity_type)
+     apply(rule_tac n="arity(q)" in nat_into_Ord,erule arity_type,simp)
+  apply(subgoal_tac "arity(q)\<le>n",simp)
+  apply(rule conjunct2,rule  iffD1,rule Un_least_lt_iff,auto,(rule nat_into_Ord,erule arity_type)+)
   apply(rename_tac m g)
   apply(erule_tac x="succ(m)" in allE,rule impE,assumption,simp)
   apply (clarsimp)
   apply(rule_tac x="perm_n(m,g)"  in allE,assumption,rule impE)
-  apply (assumption,simp,erule_tac P="arity(p) \<le> m" in impE)
+  apply (assumption,simp,erule_tac P="arity(p) \<le> succ(m)" in impE)
   apply (simp,auto)
-  apply(rule pred_le2,auto)
+  apply(rule pred_le2,auto,erule arity_type)
 done
 
-(*
-consts   rename :: "i=>i"
-primrec
-  "rename(Member(x,y)) =
-      (\<lambda> n \<in> nat . \<lambda>f \<in> bij(n,n). Member (f`x, f`y))"
+lemma ren_tc2 : "p \<in> formula \<Longrightarrow> n \<in> nat \<Longrightarrow> f \<in> bij(n,n) \<Longrightarrow> arity(p) \<le> n \<Longrightarrow> rename(p)`n`f \<in> formula"
+  by (insert ren_tc,auto)
+  
+lemma Nand_equiv : "\<lbrakk> env \<in> list(M) ; env' \<in> list(M) ; 
+  p \<in> formula;q \<in> formula ; p' \<in> formula ; q' \<in> formula ;
+  sats(M,p,env) \<longleftrightarrow> sats(M,p',env') ;
+sats(M,q,env) \<longleftrightarrow> sats(M,q',env') \<rbrakk> \<Longrightarrow>
+sats(M,Nand(p,q),env) \<longleftrightarrow> sats(M,Nand(p',q'),env')" 
+  by(auto)
 
-  "rename(Equal(x,y)) =
-      (\<lambda> n \<in> nat . \<lambda>f \<in> bij(n,n). Equal (f`x, f`y))"
+lemma Forall_equiv : "\<lbrakk> env \<in> list(M) ; env' \<in> list(M) ; 
+  p \<in> formula; p' \<in> formula ; \<And> a . a  \<in> M  \<longrightarrow>
+  (sats(M,p,Cons(a,env)) \<longleftrightarrow> sats(M,p',Cons(a,env')))  \<rbrakk> \<Longrightarrow>
+sats(M,Forall(p),env) \<longleftrightarrow> sats(M,Forall(p'),env')" 
+  by(simp)
 
-  "rename(Nand(p,q)) =
-      (\<lambda> n \<in> nat . \<lambda>f \<in> bij(n,n). Nand (rename(p)`n`f, rename(q)`n`f))"
+    
+lemma arity_meml : "l \<in> nat \<Longrightarrow> Member(x,y) \<in> formula \<Longrightarrow> arity(Member(x,y)) \<le> l \<Longrightarrow> x \<in> l"
+  by(simp,rule subsetD,rule le_imp_subset,assumption,simp)  
+lemma arity_memr : "l \<in> nat \<Longrightarrow> Member(x,y) \<in> formula \<Longrightarrow> arity(Member(x,y)) \<le> l \<Longrightarrow> y \<in> l"
+  by(simp,rule subsetD,rule le_imp_subset,assumption,simp)  
+lemma arity_eql : "l \<in> nat \<Longrightarrow> Equal(x,y) \<in> formula \<Longrightarrow> arity(Equal(x,y)) \<le> l \<Longrightarrow> x \<in> l"
+  by(simp,rule subsetD,rule le_imp_subset,assumption,simp)  
+lemma arity_eqr : "l \<in> nat \<Longrightarrow> Equal(x,y) \<in> formula \<Longrightarrow> arity(Equal(x,y)) \<le> l \<Longrightarrow> y \<in> l"
+  by(simp,rule subsetD,rule le_imp_subset,assumption,simp)  
+lemmas mem_sat_ch = mem_iff_sats [THEN iffD2]        
+lemmas mem_sat_chr = mem_iff_sats [THEN iffD1]        
 
-  "rename(Forall(p)) =
-      (\<lambda> n \<in> nat . \<lambda>f \<in> bij(n,n). Forall (rename(p) `succ(n)` perm_n(n,f)))"
-*)
-*)
-definition
-  swap_var :: "[i , i] \<Rightarrow> i" where
-  "swap_var(i,n) == if i=n then succ(i) else (if i=succ(n) then n else i)"
+lemma mem_iff_sats2:
+  "env\<in>list(A) \<Longrightarrow> sats(A, Member(i,j), env) \<Longrightarrow> nth(i,env) \<in> nth(j,env)"
+by (insert satisfies.simps(1),simp)
 
-lemma swap_var_type [TC] : 
-  "\<lbrakk> i \<in> nat ; n \<in> nat \<rbrakk> \<Longrightarrow> swap_var(i,n) \<in> nat"
-  by (simp add:swap_var_def)
+lemma renSat : "p \<in> formula \<Longrightarrow> (\<forall> env . env \<in> list(M) \<longrightarrow>
+         (\<forall> f . f \<in> bij(length(env),length(env)) \<longrightarrow>
+        arity(p) \<le> length(env) \<longrightarrow>
+         sats(M,p,env) \<longleftrightarrow> 
+         sats(M,rename(p)`length(env)`converse(f),perm_list(f,env))))"
+   apply (induct_tac p,(rule allI,(rule impI)+)+)
+      apply (subst ren_mem,assumption+,erule length_type)
+       apply(erule bij_converse_bij,rule iffI)
+     apply(rule iffD1,rule_tac x="nth(x,env)" and y="nth(y,env)" in mem_iff_sats)
+          apply(rule nth_perm,assumption+,rule arity_meml,erule length_type,simp,assumption)
+         apply(rule nth_perm,assumption+,rule arity_memr,erule length_type,simp,assumption)
+        apply(erule perm_list_tc,assumption,simp)
+     apply(rule iffD1,rule_tac i="x" and j="y" and x="nth(x,env)" and y="nth(y,env)" in mem_iff_sats,simp+)
+     apply(rule mem_iff_sats[THEN iffD2]) prefer 4 apply(assumption)
+        apply(rule nth_perm,assumption+,rule_tac y="y" in arity_meml,erule length_type,simp+)
+        apply(rule nth_perm,assumption+,rule_tac x="x" in arity_memr,erule length_type,simp+)
+      apply(erule perm_list_tc,assumption)
+    apply (rule allI,(rule impI)+)+
+     apply (subst ren_eq,assumption+,erule length_type)
+       apply(erule bij_converse_bij,rule iffI)
+      apply(rule iffD1,rule_tac x="nth(x,env)" and y="nth(y,env)" in equal_iff_sats)
+     apply(rule nth_perm,assumption+,rule arity_eql,erule length_type,simp,assumption)
+      apply(rule nth_perm,assumption+,rule arity_eqr,erule length_type,simp,assumption)
+      apply(erule perm_list_tc,assumption,simp)
+     apply(rule iffD1,rule_tac i="x" and j="y" and x="nth(x,env)" and y="nth(y,env)" in equal_iff_sats,simp+)
+     apply(rule equal_iff_sats[THEN iffD2]) prefer 4 apply(assumption)
+        apply(rule nth_perm,assumption+,rule_tac y="y" in arity_meml,erule length_type,simp+)
+       apply(rule nth_perm,assumption+,rule_tac x="x" in arity_memr,erule length_type,simp+)
+      apply(erule perm_list_tc,assumption)
+     apply (rule allI,(rule impI)+)+
+    apply (subst ren_nand,assumption+,erule length_type)
+    apply(erule bij_converse_bij)
+    apply(subgoal_tac "arity(q) \<le> length(env)")
+    prefer 2      
+      apply(simp,rule_tac j="arity(Nand(p,q))" in le_trans,simp,rule Un_upper2_le,
+           (rule nat_into_Ord,rule arity_type,assumption)+,simp)
+    apply(subgoal_tac "arity(p) \<le> length(env)")
+    prefer 2
+      apply(simp,rule_tac j="arity(Nand(p,q))" in le_trans,simp,rule Un_upper1_le,
+           (rule nat_into_Ord,rule arity_type,assumption)+,simp)
+     apply(rule Nand_equiv,simp+,rule perm_list_tc,simp+,rule ren_tc2,simp+,erule length_type)
+         apply(erule bij_converse_bij,assumption) 
+           apply(rule ren_tc2,simp+,erule length_type,erule bij_converse_bij,assumption) 
+      apply (simp,simp)
+    apply (rule allI,(rule impI)+)+
+  apply(subst ren_forall,assumption,erule length_type,erule bij_converse_bij )
+ apply(rule Forall_equiv,simp+,erule perm_list_tc,assumption+)
+  apply(rule ren_tc2,simp+,erule length_type,rule perm_n_bij,erule length_type)
+  apply(erule bij_converse_bij,rule le_trans)
+  prefer 2 apply (rule succ_leI,assumption,simp,rule succpred_leI,erule arity_type)
+  apply(rule impI)
+  apply(subgoal_tac "Cons(a,perm_list(f,env)) = perm_list(perm_n(length(env),f),Cons(a,env))",simp)
+  apply(erule_tac x="Cons(a,env)" in allE)
+  apply(subgoal_tac "Cons(a,env) \<in> list(M)")
+  apply(subgoal_tac "perm_n(length(env),f) \<in> bij(length(Cons(a,env)),length(Cons(a,env)))")
+  apply(erule impE,assumption,erule_tac x="perm_n(length(env),f)" in allE)
+  apply(erule impE,assumption)
+    apply(erule impE)
+  apply(rule_tac j="succ(pred(arity(p)))" in le_trans)
+   apply (rule succpred_leI,erule arity_type,simp,simp+)
+    prefer 3 apply(simp)
+   prefer 2 apply(simp,rule perm_n_bij,erule length_type,assumption)
+   apply(subst conv_perm,erule length_type,simp,rule iff_refl)
+  apply(subst perm_list_eq,simp+)
+done
 
-consts swap_suc :: "i\<Rightarrow>i" 
-primrec
-  "swap_suc(Member(x,y)) =
-    (\<lambda> n \<in> nat . Member(swap_var(x,n),swap_var(y,n)))"
-  "swap_suc(Equal(x,y)) = 
-    (\<lambda> n \<in> nat . Equal(swap_var(x,n),swap_var(y,n)))"
-  "swap_suc(Nand(p,q)) =
-    (\<lambda> n \<in> nat . Nand(swap_suc(p)`n,swap_suc(q)`n))"
-  "swap_suc(Forall(p)) =
-    (\<lambda> n \<in> nat . Forall(swap_suc(p)`(succ(n))))"
+lemma sat_env_eq : "p \<in> formula \<Longrightarrow> env \<in> list(M) \<Longrightarrow> env'\<in> list(M) \<Longrightarrow>
+   env=env' \<Longrightarrow>         sats(M,p,env) \<longleftrightarrow> sats(M,p,env')"
+  by(auto)
+    
+definition 
+  swap01 :: "i" where
+  "swap01 == \<lambda> n \<in> 2 . if n=0 then 1 else 0"
 
-lemma swap_suc_type [TC] : 
-  "\<lbrakk> \<phi> \<in> formula  \<rbrakk> \<Longrightarrow> swap_suc(\<phi>) \<in> nat \<rightarrow> formula"
-  by (induct_tac \<phi>,simp_all)
+lemma swap01_bij : "swap01 \<in> bij(2,2)"
+  by(unfold swap01_def,rule_tac  d="\<lambda> n. if n =0 then 1 else 0" in lam_bijective,auto)
 
-lemma sats_swap_suc : 
-  "\<lbrakk> \<phi> \<in> formula ; n \<in> nat ; env \<in> list(M) ; env' \<in> list(M) ; n = length(env) \<rbrakk> \<Longrightarrow> 
-    sats(M,\<phi>,env@[a,b]@env') \<longleftrightarrow> sats(M,swap_suc(\<phi>)`n,env@[b,a]@env')"
-  sorry
+definition ext_fun :: "[i,i] \<Rightarrow> i" where
+    "ext_fun(f,m) == \<lambda> n \<in> m . if n <2 then f`n else n"
+
+lemma swap_0 [simp]: "swap01`0 = 1"
+    by(unfold swap01_def,simp,auto)
+lemma swap_1 [simp]: "swap01`1 = 0"
+    by(unfold swap01_def,simp)
+lemma swap_auto [simp] : "x < 2 \<Longrightarrow> swap01`(swap01`x) = x" 
+  by(case_tac "x\<le>0",simp+,subgoal_tac "x=1",simp,rule leE[of "x" "1"],simp,auto)
+      
+lemma ext_fun_bij : "m \<in> nat \<Longrightarrow> 2<m \<Longrightarrow> ext_fun(swap01,m) \<in> bij(m,m)"
+  apply(unfold ext_fun_def)
+  apply(rule_tac  d="\<lambda> n. if n < 2 then swap01`n else n" in lam_bijective)
+   apply(case_tac "x<2",simp,rule ltD,rule_tac j="2" in lt_trans,rule ltI)
+   apply(rule apply_type,rule bij_is_fun,rule swap01_bij,rule ltD,simp,simp+)
+    apply(rule impI,rule ltD,rule_tac j="2" in lt_trans,rule ltI)
+    apply(rule apply_type,rule bij_is_fun,rule swap01_bij,rule ltD,simp,simp+)
+   apply(auto,subgoal_tac "swap01`x \<le> 1",simp,rule ltI,rule apply_type)
+   apply(rule bij_is_fun,rule swap01_bij,erule ltD,simp)
+   apply(subgoal_tac "swap01`y \<le> 1",simp,rule ltI,rule apply_type)
+   apply(rule bij_is_fun,rule swap01_bij,erule ltD,simp)
+done
+lemma ext_fun_bije : "m \<in> nat \<Longrightarrow> 2\<le>m \<Longrightarrow> ext_fun(swap01,m) \<in> bij(m,m)"
+  apply(erule leE,rule ext_fun_bij,simp+)
+  apply(subgoal_tac "m=2",thin_tac "2=m",simp,unfold ext_fun_def)
+  apply(rule_tac d="\<lambda> n . swap01`n" in lam_bijective,auto)
+done
+
+lemma ext_fun_swap0 [simp]: "m \<in> nat \<Longrightarrow> 2\<le>m \<Longrightarrow> ext_fun(swap01,m)`0=1"
+  by(insert swap_0,unfold ext_fun_def,simp,rule ltD,rule_tac j="1"  in lt_trans,auto)
+    
+lemma ext_fun_swap1 [simp]: "m \<in> nat \<Longrightarrow> 2\<le>m \<Longrightarrow> ext_fun(swap01,m)`1=0"  
+ by(insert swap_1,unfold ext_fun_def,simp)
+  
+lemma ext_fun_swap_n : "m \<in> nat \<Longrightarrow> 1<n \<Longrightarrow> n \<in> m \<Longrightarrow> ext_fun(swap01,m)`n=n"  
+  by(unfold ext_fun_def,simp,rule impI,rule_tac i="n" and j="2" in ltE,simp,auto)
+
+lemma ext_swap_i0: "m \<in> nat \<Longrightarrow> n \<in> m \<Longrightarrow> 2\<le>m \<Longrightarrow> ext_fun(swap01,m)`n=1 \<Longrightarrow> n=0"
+  by(rule inj_apply_equality,rule bij_is_inj,rule ext_fun_bije,simp+,rule ltD,rule lt_trans,rule nat_0_le,auto)
+
+lemma ext_swap_i1: "m \<in> nat \<Longrightarrow> n \<in> m \<Longrightarrow> 2\<le>m \<Longrightarrow> ext_fun(swap01,m)`n=0 \<Longrightarrow> n=1"
+  by(rule inj_apply_equality,rule bij_is_inj,rule ext_fun_bije,simp+,erule ltD)
+
+lemma ext_wap_in : "m \<in> nat \<Longrightarrow> 1<n \<Longrightarrow> n \<in> m \<Longrightarrow> ext_fun(swap01,m)`n=j \<Longrightarrow> j=n"  
+  apply(rule inj_apply_equality,rule bij_is_inj,rule ext_fun_bije,simp+,rule lt_trans,simp)
+  prefer 2 apply(subst (asm) ext_fun_swap_n,simp+,erule ltI,simp)
+  apply(subst (asm) ext_fun_swap_n,simp+)
+  done
+    
+  
+lemma conv_swap : "m\<in>nat \<Longrightarrow> 2\<le> m \<Longrightarrow> converse(ext_fun(swap01,m)) = ext_fun(swap01,m)"
+  apply(rule fun_extension,rule bij_is_fun,rule bij_converse_bij,rule ext_fun_bije,simp+)
+  apply(rule bij_is_fun,rule ext_fun_bije,simp+)
+  apply(case_tac "x<2")
+  apply(rule leE[of _ "1"],assumption,simp,rule left_inverse_eq)  
+  apply(rule bij_is_inj,rule ext_fun_bije,simp+,rule ltD,simp)
+  apply(simp)
+  apply(rule left_inverse_eq)  
+  apply(rule bij_is_inj,rule ext_fun_bije,simp+,rule ltD,rule lt_trans)
+  prefer 2 apply(assumption,simp)
+  apply(subgoal_tac "2\<le>x")
+  apply(rule left_inverse_eq)  
+  apply(rule bij_is_inj,rule ext_fun_bije,simp+)
+  apply(subst ext_fun_swap_n,simp+)+
+  apply(rule_tac not_le_iff_lt[THEN iffD1],rule nat_into_Ord,erule in_n_in_nat,simp+)
+done
+    
+lemma pred0E : "i \<in> nat \<Longrightarrow> pred(i) = 0 \<Longrightarrow> i = 1 | i = 0"
+  by(rule natE,simp+)
+  
+lemma swap_env : "l \<in> list(M) \<Longrightarrow> a \<in> M \<Longrightarrow> b \<in> M \<Longrightarrow> 
+  perm_list(ext_fun(swap01,succ(succ(length(l)))),Cons(a,(Cons(b,l)))) =
+  Cons(b,Cons(a,l))"
+  apply(subgoal_tac 
+  "ext_fun(swap01, succ(succ(length(l)))) \<in> bij(length(Cons(a, Cons(b, l))), length(Cons(a, Cons(b, l))))")
+prefer 2 
+  apply(simp,rule_tac m="succ(succ(length(l)))" in ext_fun_bije,simp+,rule length_type,simp+)
+  apply(rule nat_0_le,rule length_type,simp+)
+  apply(rule nth_equalityI,rule perm_list_tc,simp+,subst perm_list_length,simp+)
+  apply(subst (asm) perm_list_length,simp+)
+  apply(case_tac "i=0",simp)
+  apply(subst nth_perm1,simp+,rule ltD)
+  apply(rule nat_0_le,simp,erule length_type)
+  apply(subst ext_fun_swap0,simp,erule length_type,simp)
+  apply(rule nat_0_le,erule length_type,simp)
+  apply(case_tac "i=1",simp) 
+  apply(subst nth_perm1,simp+,rule ltD,simp)
+  apply(subst ext_fun_swap1,simp,erule length_type,simp+)
+  apply(subgoal_tac "\<exists> j . i = succ(succ(j))")
+  apply(erule exE)
+  apply(subst nth_perm1,simp+,rule ltD,simp)
+  apply(subst ext_fun_swap_n,simp,erule length_type,simp,erule ltD)
+  apply(simp,rule_tac x="pred(pred(i))" in exI)
+  apply(subst succ_pred_eq,erule pred_type)
+  prefer 2 apply(subst succ_pred_eq,simp+,auto)
+  apply(drule pred0E,simp,auto)
+done
 
 definition
   swap_0_1 :: "i \<Rightarrow> i" where
-  "swap_0_1(\<phi>) == swap_suc(\<phi>)`0"
+  "swap_0_1(\<phi>) == \<lambda> m \<in> nat . rename(\<phi>)`m`ext_fun(m,swap01)"  
 
-lemma [TC] : "\<phi> \<in> formula \<Longrightarrow> swap_0_1(\<phi>) \<in> formula"
-  by (simp add: swap_0_1_def)
-  
-
-lemma sats_swap_0_1 :
-  "\<lbrakk> \<phi> \<in> formula ; env \<in> list(M) ; a \<in> M ; b \<in> M\<rbrakk> \<Longrightarrow>
-  sats(M,swap_0_1(\<phi>),Cons(a,Cons(b,env))) \<longleftrightarrow> 
-  sats(M,\<phi>,Cons(b,Cons(a,env)))"
-  sorry
-
-(* sats(M, swap_0_1(\<phi>),Cons(xb, Cons(x, Cons(A, env)))*)
-
-(*
-lemma renSat : "p \<in> formula \<Longrightarrow> (\<forall> f . f \<in> bij(arity(p),arity(p)) \<longrightarrow> 
-        arity(p) \<le> length(env) \<longrightarrow>  (* es necesario? *)
-        sats(M,p,env) \<longrightarrow> 
-        sats(M,rename(p)`f,perm_list(converse(f),env,length(env))))"
-  apply (induct_tac p)
-     apply (simp)
-  sorry
+(*        
+sats(M,p,env) \<longleftrightarrow> sats(M,rename(p)`length(env)`converse(f),perm_list(f,env))))"
 *)
-end
+lemma ren_sat : "p \<in> formula \<Longrightarrow> env \<in> list(M) \<Longrightarrow> f \<in> bij(length(env),length(env)) \<Longrightarrow>
+        arity(p) \<le> length(env) \<Longrightarrow>
+        sats(M,p,env) \<longleftrightarrow> 
+        sats(M,rename(p)`length(env)`converse(f),perm_list(f,env))"
+ by(insert renSat,simp)
+  
+lemma sats_swap_0_1 :
+  "\<lbrakk> \<phi> \<in> formula ; env \<in> list(M) ; a \<in> M ; b \<in> M ; arity(\<phi>) \<le> succ(succ(length(env))) \<rbrakk> \<Longrightarrow>
+  sats(M,\<phi>,Cons(b,Cons(a,env))) \<longleftrightarrow>
+  sats(M,rename(\<phi>)`succ(succ(length(env)))`ext_fun(swap01,succ(succ(length(env)))),Cons(a,Cons(b,env)))"
+  apply(subst swap_env[symmetric,of "env" "M" "b" "a"],simp+)
+  apply(rule iff_trans)
+   apply(rule_tac f="ext_fun(swap01,succ(succ(length(env))))" in ren_sat,simp+)
+  apply(rule ext_fun_bije,simp+,erule length_type,simp,rule nat_0_le,erule length_type,simp)
+  apply(subst conv_swap,simp,erule length_type,simp,rule nat_0_le,erule length_type,simp)
+done
